Refactor.
Kinded subtyping, better file structure, more setoid stuff, reorganize imports.

theories/logrel/model.v
@@ -1,149 +1,88 @@
-From iris.heap_lang Require Export lifting metatheory.
-From iris.base_logic.lib Require Import invariants.
-From iris.heap_lang Require Import notation proofmode.
-From actris.channel Require Import proto proofmode.
+From iris.algebra Require Export ofe.
+From actris.channel Require Export channel.
 
-Record lty_raw Σ := Lty {
-  lty_car :> val → iProp Σ;
-}.
-Arguments Lty {_} _%I.
-Arguments lty_car {_} _ _ : simpl never.
+Inductive kind := tty_kind | sty_kind.
+Instance kind_eq_dec : EqDecision kind.
+Proof. solve_decision. Defined.
+Instance kind_inhabited : Inhabited kind := populate tty_kind.
 
-(* The COFE structure on semantic types *)
-Section lty_ofe.
-  Context `{Σ : gFunctors}.
-
-  (* Equality of semantic types is extensional equality *)
-  Instance lty_equiv : Equiv (lty_raw Σ) := λ A B, ∀ w, A w ≡ B w.
-  Instance lty_dist : Dist (lty_raw Σ) := λ n A B, ∀ w, A w ≡{n}≡ B w.
-
-  (* OFE and COFE structure is taken from isomorphism with val -d> iProp Σ *)
-  Lemma lty_ofe_mixin : OfeMixin (lty_raw Σ).
-  Proof. by apply (iso_ofe_mixin (lty_car : _ → val -d> _)). Qed.
-  Canonical Structure lty_rawO := OfeT (lty_raw Σ) lty_ofe_mixin.
-
-  Global Instance lty_cofe : Cofe lty_rawO.
-  Proof. by apply (iso_cofe (@Lty _ : (val -d> _) → lty_rawO) lty_car). Qed.
-
-  Global Instance lty_inhabited : Inhabited (lty_raw Σ) := populate (Lty inhabitant).
-
-  Global Instance lty_car_ne n : Proper (dist n ==> (=) ==> dist n) lty_car.
-  Proof. by intros A A' ? w ? <-. Qed.
-  Global Instance lty_car_proper : Proper ((≡) ==> (=) ==> (≡)) lty_car.
-  Proof. by intros A A' ? w ? <-. Qed.
-
-  Global Instance lty_ne n : Proper (pointwise_relation _ (dist n) ==> dist n) Lty.
-  Proof. by intros ???. Qed.
-  Global Instance lty_proper : Proper (pointwise_relation _ (≡) ==> (≡)) Lty.
-  Proof. by intros ???. Qed.
-End lty_ofe.
-
-Arguments lty_rawO : clear implicits.
-
-Record lsty_raw Σ := Lsty {
-  lsty_car :> iProto Σ;
-}.
+(** Use [Variant] to supress generation of induction schemes *)
+Variant lty Σ : kind → Type :=
+  | Ltty : (val → iProp Σ) → lty Σ tty_kind
+  | Lsty : iProto Σ → lty Σ sty_kind.
+Arguments Ltty {_} _%I.
 Arguments Lsty {_} _%proto.
+
+Bind Scope lty_scope with lty.
+Delimit Scope lty_scope with lty.
+
+Notation ltty Σ := (lty Σ tty_kind).
+Notation lsty Σ := (lty Σ sty_kind).
+
+Definition ltty_car {Σ} (A : ltty Σ) : val → iProp Σ :=
+  match A with Ltty A => A | Lsty _ => () end.
+Definition lsty_car {Σ} (p : lsty Σ) : iProto Σ :=
+  match p with Ltty _ => () | Lsty p => p end.
+Arguments ltty_car {_} _ _ : simpl never.
 Arguments lsty_car {_} _ : simpl never.
 
-Section lsty_ofe.
-  Context `{Σ : gFunctors}.
-
-  Instance lsty_equiv : Equiv (lsty_raw Σ) :=
-    λ P Q, lsty_car P ≡ lsty_car Q.
-  Instance lsty_dist : Dist (lsty_raw Σ) :=
-    λ n P Q, lsty_car P ≡{n}≡ lsty_car Q.
-
-  Lemma lsty_ofe_mixin : OfeMixin (lsty_raw Σ).
-  Proof. by apply (iso_ofe_mixin (lsty_car : _ → iProto _)). Qed.
-  Canonical Structure lsty_rawO := OfeT (lsty_raw Σ) lsty_ofe_mixin.
-
-  Global Instance lsty_cofe : Cofe lsty_rawO.
-  Proof. by apply (iso_cofe (@Lsty _ : _ → lsty_rawO) lsty_car). Qed.
-
-  Global Instance lsty_inhabited : Inhabited (lsty_raw Σ) :=
-    populate (Lsty inhabitant).
-
-  Global Instance lsty_car_ne : NonExpansive lsty_car.
-  Proof. intros n A A' H. exact H. Qed.
-
-  Global Instance lsty_car_proper : Proper ((≡) ==> (≡)) lsty_car.
-  Proof. intros A A' H. exact H. Qed.
-
-  Global Instance Lsty_ne : NonExpansive Lsty.
-  Proof. solve_proper. Qed.
-
-  Global Instance Lsty_proper : Proper ((≡) ==> (≡)) Lsty.
-  Proof. solve_proper. Qed.
-End lsty_ofe.
-
-Arguments lsty_rawO : clear implicits.
-
-Inductive kind :=
-  | ty_kind | sty_kind.
-
-Definition kind_interp (k : kind) Σ : Type :=
+Instance lty_inhabited Σ k : Inhabited (lty Σ k) := populate $
   match k with
-  | ty_kind => lty_raw Σ
-  | sty_kind => lsty_raw Σ
+  | tty_kind => Ltty inhabitant
+  | lty_kind => Lsty inhabitant
   end.
 
-Notation lty Σ := (kind_interp ty_kind Σ).
-Notation lsty Σ := (kind_interp sty_kind Σ).
-Bind Scope kind_scope with kind_interp.
-Delimit Scope kind_scope with kind.
-
-(* The COFE structure on semantic types *)
 Section lty_ofe.
-  Context `{Σ : gFunctors}.
+  Context {Σ : gFunctors}.
 
-  Instance kind_interp_equiv k : Equiv (kind_interp k Σ) :=
+  Instance lty_equiv k : Equiv (lty Σ k) :=
     match k with
-    | ty_kind => λ A B, ∀ w, A w ≡ B w
+    | tty_kind => λ A B, ∀ w, ltty_car A w ≡ ltty_car B w
     | lty_kind => λ S T, lsty_car S ≡ lsty_car T
     end.
-  Instance kind_interp_dist k : Dist (kind_interp k Σ) :=
+  Instance lty_dist k : Dist (lty Σ k) :=
     match k with
-    | ty_kind =>  λ n A B, ∀ w, A w ≡{n}≡ B w
+    | tty_kind => λ n A B, ∀ w, ltty_car A w ≡{n}≡ ltty_car B w
     | lty_kind => λ n S T, lsty_car S ≡{n}≡ lsty_car T
     end.
 
-  Lemma kind_interp_mixin k : OfeMixin (kind_interp k Σ).
+  Lemma lty_mixin k : OfeMixin (lty Σ k).
   Proof.
     destruct k.
-    - by apply (iso_ofe_mixin (lty_car : _ → val -d> _)).
+    - by apply (iso_ofe_mixin (ltty_car : _ → val -d> _)).
     - by apply (iso_ofe_mixin (lsty_car : _ → iProto _)).
   Qed.
-  Canonical Structure kind_interpO k :=
-    OfeT (kind_interp k Σ) (kind_interp_mixin k).
+  Canonical Structure ltyO k := OfeT (lty Σ k) (lty_mixin k).
 
-  Global Instance kind_interp_cofe k : Cofe (kind_interpO k).
+  Global Instance lty_cofe k : Cofe (ltyO k).
   Proof.
     destruct k.
-    - by apply (iso_cofe (@Lty _ : (val -d> _) → (kind_interpO ty_kind)) lty_car).
-    - by apply (iso_cofe (@Lsty _ : _ → (kind_interpO sty_kind)) lsty_car).
+    - by apply (iso_cofe (Ltty : (val -d> _) → _) ltty_car).
+    - by apply (iso_cofe Lsty lsty_car).
   Qed.
 
-  Global Instance kind_interp_inhabited k : Inhabited (kind_interp k Σ).
-  Proof.
-    destruct k.
-    - apply (populate (Lty inhabitant)).
-    - apply (populate (Lsty inhabitant)).
-  Qed.
+  Global Instance ltty_car_ne n : Proper (dist n ==> (=) ==> dist n) ltty_car.
+  Proof. by intros A A' ? w ? <-. Qed.
+  Global Instance ltty_car_proper : Proper ((≡) ==> (=) ==> (≡)) ltty_car.
+  Proof. by intros A A' ? w ? <-. Qed.
+  Global Instance lsty_car_ne : NonExpansive lsty_car.
+  Proof. intros n A A' H. exact H. Qed.
+  Global Instance lsty_car_proper : Proper ((≡) ==> (≡)) lsty_car.
+  Proof. intros A A' H. exact H. Qed.
 
+  Global Instance Ltty_ne n : Proper (pointwise_relation _ (dist n) ==> dist n) Ltty.
+  Proof. by intros ???. Qed.
+  Global Instance Ltty_proper : Proper (pointwise_relation _ (≡) ==> (≡)) Ltty.
+  Proof. by intros ???. Qed.
+  Global Instance Lsty_ne : NonExpansive Lsty.
+  Proof. solve_proper. Qed.
+  Global Instance Lsty_proper : Proper ((≡) ==> (≡)) Lsty.
+  Proof. solve_proper. Qed.
 End lty_ofe.
 
-Arguments kind_interpO : clear implicits.
+Arguments ltyO : clear implicits.
+Notation lttyO Σ := (ltyO Σ tty_kind).
+Notation lstyO Σ := (ltyO Σ sty_kind).
 
-Notation ltyO Σ := (kind_interpO Σ ty_kind).
-Notation lstyO Σ := (kind_interpO Σ sty_kind).
-
-(* Typing for operators *)
-Class LTyUnboxed {Σ} (A : lty Σ) :=
-  lty_unboxed v : A v -∗ ⌜ val_is_unboxed v ⌝.
-
-Class LTyUnOp {Σ} (op : un_op) (A B : lty Σ) :=
-  lty_un_op v : A v -∗ ∃ w, ⌜ un_op_eval op v = Some w ⌝ ∗ B w.
-
-Class LTyBinOp {Σ} (op : bin_op) (A1 A2 B : lty Σ) :=
-  lty_bin_op v1 v2 : A1 v1 -∗ A2 v2 -∗ ∃ w, ⌜ bin_op_eval op v1 v2 = Some w ⌝ ∗ B w.
+Definition lty_rec {Σ k} (C : lty Σ k → lty Σ k) `{!Contractive C} : lty Σ k :=
+  fixpoint C.
