theories/logrel/session_types.v
@@ -1,121 +1,70 @@
+From iris.algebra Require Export gmap.
 From actris.logrel Require Export model.
-From iris.algebra Require Import gmap.
-From iris.heap_lang Require Export lifting metatheory.
-From iris.base_logic.lib Require Import invariants.
-From iris.heap_lang Require Import notation proofmode.
-From actris.channel Require Import proto proofmode.
+From actris.channel Require Export channel.
 
-Section protocols.
-  Context `{heapG Σ, protoG Σ}.
+Definition lty_end {Σ} : lsty Σ := Lsty END.
 
-  Definition lsty_end : lsty Σ := Lsty END.
+Definition lty_message {Σ} (a : action) (A : ltty Σ) (S : lsty Σ) : lsty Σ :=
+  Lsty (<a> v, MSG v {{ ltty_car A v }}; lsty_car S).
 
-  Definition lsty_message (a : action) (A : lty Σ) (S : lsty Σ) : lsty Σ :=
-    Lsty (<a> v, MSG v {{ A v }}; lsty_car S).
+Definition lty_choice {Σ} (a : action) (Ss : gmap Z (lsty Σ)) : lsty Σ :=
+  Lsty (<a> x : Z, MSG #x {{ ⌜is_Some (Ss !! x)⌝ }}; lsty_car (Ss !!! x)).
 
-  Definition lsty_send (A : lty Σ) (S : lsty Σ) : lsty Σ :=
-    lsty_message Send A S.
-  Definition lsty_recv (A : lty Σ) (S : lsty Σ) : lsty Σ :=
-    lsty_message Recv A S.
+Definition lty_dual {Σ} (S : lsty Σ) : lsty Σ :=
+  Lsty (iProto_dual (lsty_car S)).
+Definition lty_app {Σ} (S1 S2 : lsty Σ) : lsty Σ :=
+  Lsty (lsty_car S1 <++> lsty_car S2).
 
-  Definition lsty_choice (a : action) (Ss : gmap Z (lsty Σ)) : lsty Σ :=
-    Lsty (<a> x : Z, MSG #x {{ ⌜is_Some (Ss !! x)⌝ }}; lsty_car (Ss !!! x)).
+Instance: Params (@lty_message) 2 := {}.
+Instance: Params (@lty_choice) 2 := {}.
+Instance: Params (@lty_dual) 1 := {}.
+Instance: Params (@lty_app) 1 := {}.
 
-  Definition lsty_select (Ss : gmap Z (lsty Σ)) : lsty Σ :=
-    lsty_choice Send Ss.
-  Definition lsty_branch (Ss : gmap Z (lsty Σ)) : lsty Σ :=
-    lsty_choice Recv Ss.
+Notation "'END'" := lty_end : lty_scope.
+Notation "<!!> A ; S" :=
+  (lty_message Send A S) (at level 20, A, S at level 200) : lty_scope.
+Notation "<??> A ; S" :=
+  (lty_message Recv A S) (at level 20, A, S at level 200) : lty_scope.
+Notation lty_select := (lty_choice Send).
+Notation lty_branch := (lty_choice Recv).
+Infix "<++>" := lty_app (at level 60) : lty_scope.
+Notation "( S <++>.)" := (lty_app S) (only parsing) : lty_scope.
+Notation "(.<++> T )" := (λ S, lty_app S T) (only parsing) : lty_scope.
 
-  Definition lsty_rec1 (C : lsty Σ → lsty Σ) `{!Contractive C}
-    (rec : lsty Σ) : lsty Σ := Lsty (C rec).
-  Instance lsty_rec1_contractive C `{!Contractive C} : Contractive (lsty_rec1 C).
-  Proof. solve_contractive. Qed.
-  Definition lsty_rec (C : lsty Σ → lsty Σ) `{!Contractive C} : lsty Σ :=
-    fixpoint (lsty_rec1 C).
+Section session_types.
+  Context {Σ : gFunctors}.
 
-  Definition lsty_dual (S : lsty Σ) : lsty Σ :=
-    Lsty (iProto_dual S).
-
-  Definition lsty_app (S1 S2 : lsty Σ) : lsty Σ :=
-    Lsty (S1 <++> S2).
-End protocols.
-
-Section Propers.
-  Context `{heapG Σ, protoG Σ}.
-
-  Global Instance lsty_message_ne a : NonExpansive2 (@lsty_message Σ a).
+  Global Instance lty_message_ne a : NonExpansive2 (@lty_message Σ a).
   Proof. intros n A A' ? S S' ?. by apply iProto_message_ne; simpl. Qed.
-  Global Instance lsty_message_proper a :
-    Proper ((≡) ==> (≡) ==> (≡)) (@lsty_message Σ a).
+  Global Instance lty_message_proper a :
+    Proper ((≡) ==> (≡) ==> (≡)) (@lty_message Σ a).
   Proof. apply ne_proper_2, _. Qed.
-  Global Instance lsty_message_contractive n a :
-    Proper (dist_later n ==> dist_later n ==> dist n) (@lsty_message Σ a).
+  Global Instance lty_message_contractive n a :
+    Proper (dist_later n ==> dist_later n ==> dist n) (@lty_message Σ a).
   Proof.
     intros A A' ? S S' ?.
     apply iProto_message_contractive; simpl; done || by destruct n.
   Qed.
 
-  Global Instance lsty_send_ne : NonExpansive2 (@lsty_send Σ).
-  Proof. solve_proper. Qed.
-  Global Instance lsty_send_proper : Proper ((≡) ==> (≡) ==> (≡)) (@lsty_send Σ).
-  Proof. solve_proper. Qed.
-  Global Instance lsty_send_contractive n :
-    Proper (dist_later n ==> dist_later n ==> dist n) (@lsty_send Σ).
-  Proof. solve_contractive. Qed.
-
-  Global Instance lsty_recv_ne : NonExpansive2 (@lsty_recv Σ).
-  Proof. solve_proper. Qed.
-  Global Instance lsty_recv_proper : Proper ((≡) ==> (≡) ==> (≡)) (@lsty_recv Σ).
-  Proof. solve_proper. Qed.
-  Global Instance lsty_recv_contractive n :
-    Proper (dist_later n ==> dist_later n ==> dist n) (@lsty_recv Σ).
-  Proof. solve_contractive. Qed.
-
-  Global Instance lsty_choice_ne a : NonExpansive (@lsty_choice Σ a).
+  Global Instance lty_choice_ne a : NonExpansive (@lty_choice Σ a).
   Proof.
     intros n Ss1 Ss2 Pseq. apply iProto_message_ne; simpl; solve_proper.
   Qed.
-  Global Instance lsty_choice_proper a : Proper ((≡) ==> (≡)) (@lsty_choice Σ a).
+  Global Instance lty_choice_proper a : Proper ((≡) ==> (≡)) (@lty_choice Σ a).
   Proof. apply ne_proper. apply _. Qed.
-  Global Instance lsty_choice_contractive a : Contractive (@lsty_choice Σ a).
+  Global Instance lty_choice_contractive a : Contractive (@lty_choice Σ a).
   Proof.
     intros ? Ss1 Ss2 ?.
     apply iProto_message_contractive; destruct n; simpl; done || solve_proper.
   Qed.
 
-  Global Instance lsty_select_ne : NonExpansive (@lsty_select Σ).
+  Global Instance lty_dual_ne : NonExpansive (@lty_dual Σ).
   Proof. solve_proper. Qed.
-  Global Instance lsty_select_proper : Proper ((≡) ==> (≡)) (@lsty_select Σ).
-  Proof. solve_proper. Qed.
-  Global Instance lsty_select_contractive : Contractive (@lsty_select Σ).
-  Proof. solve_contractive. Qed.
-
-  Global Instance lsty_branch_ne : NonExpansive (@lsty_branch Σ).
-  Proof. solve_proper. Qed.
-  Global Instance lsty_branch_proper : Proper ((≡) ==> (≡)) (@lsty_branch Σ).
-  Proof. solve_proper. Qed.
-  Global Instance lsty_branch_contractive : Contractive (@lsty_branch Σ).
-  Proof. solve_contractive. Qed.
-
-  Global Instance lsty_dual_ne : NonExpansive (@lsty_dual Σ).
-  Proof. solve_proper. Qed.
-  Global Instance lsty_dual_proper : Proper ((≡) ==> (≡)) (@lsty_dual Σ).
+  Global Instance lty_dual_proper : Proper ((≡) ==> (≡)) (@lty_dual Σ).
   Proof. apply ne_proper, _. Qed.
-  Global Instance lsty_app_ne : NonExpansive2 (@lsty_app Σ).
-  Proof. solve_proper. Qed.
-  Global Instance lsty_app_proper : Proper ((≡) ==> (≡) ==> (≡)) (@lsty_app Σ).
-  Proof. apply ne_proper_2, _. Qed.
-  Global Instance lsty_app_assoc : Assoc (≡) (@lsty_app Σ).
-  Proof. intros S1 S2 S3. rewrite /lsty_app. by rewrite assoc. Qed.
-  Global Instance lsty_app_end_l : LeftId (≡) lsty_end (@lsty_app Σ).
-  Proof. intros [S]. rewrite /lsty_app. by rewrite left_id. Qed.
-  Global Instance lsty_app_end_r : RightId (≡) lsty_end (@lsty_app Σ).
-  Proof. intros [S]. rewrite /lsty_app. by rewrite right_id. Qed.
-End Propers.
 
-Notation "'END'" := lsty_end : kind_scope.
-Notation "<!!> A ; S" :=
-  (lsty_send A S) (at level 20, A, S at level 200) : kind_scope.
-Notation "<??> A ; S" :=
-  (lsty_recv A S) (at level 20, A, S at level 200) : kind_scope.
-Infix "<++>" := lsty_app (at level 60) : kind_scope.
+  Global Instance lty_app_ne : NonExpansive2 (@lty_app Σ).
+  Proof. solve_proper. Qed.
+  Global Instance lty_app_proper : Proper ((≡) ==> (≡) ==> (≡)) (@lty_app Σ).
+  Proof. apply ne_proper_2, _. Qed.
+End session_types.
