theories/logrel/term_typing_rules.v
@@ -1,87 +1,39 @@
 From stdpp Require Import pretty.
-From actris.utils Require Import switch.
-From actris.logrel Require Export model ltyping session_types.
-From actris.channel Require Import proto proofmode.
-From iris.bi.lib Require Export core.
-From iris.heap_lang Require Export lifting metatheory.
+From iris.bi.lib Require Import core.
 From iris.base_logic.lib Require Import invariants.
-From iris.heap_lang.lib Require Import assert.
-From iris.heap_lang Require Import notation proofmode lib.par spin_lock.
-
-Section types.
-  Context `{heapG Σ}.
-
-  Definition lty_unit : lty Σ := Lty (λ w, ⌜ w = #() ⌝%I).
-  Definition lty_bool : lty Σ := Lty (λ w, ∃ b : bool, ⌜ w = #b ⌝)%I.
-  Definition lty_int : lty Σ := Lty (λ w, ∃ n : Z, ⌜ w = #n ⌝)%I.
-  Definition lty_copy (A : lty Σ) : lty Σ := Lty (λ w, □ (A w))%I.
-  Definition lty_copyminus (A : lty Σ) : lty Σ := Lty (λ w, coreP (A w)).
-  Definition lty_arr (A1 A2 : lty Σ) : lty Σ := Lty (λ w,
-    ∀ v, ▷ A1 v -∗ WP w v {{ A2 }})%I.
-  (* TODO: Make a non-linear version of prod, using ∧ *)
-  Definition lty_prod (A1 A2 : lty Σ) : lty Σ := Lty (λ w,
-    ∃ w1 w2, ⌜w = (w1,w2)%V⌝ ∗ ▷ A1 w1 ∗ ▷ A2 w2)%I.
-  Definition lty_sum (A1 A2 : lty Σ) : lty Σ := Lty (λ w,
-    (∃ w1, ⌜w = InjLV w1⌝ ∗ ▷ A1 w1) ∨ (∃ w2, ⌜w = InjRV w2⌝ ∗ ▷ A2 w2))%I.
-  Definition lty_any : lty Σ := Lty (λ w, True%I).
-  Definition lty_rec_aux (C : lty Σ → lty Σ) `{!Contractive C}
-      (rec : lty Σ) : lty Σ := Lty (C rec)%I.
-  Instance lty_rec_aux_contractive C `{!Contractive C} : Contractive (lty_rec_aux C).
-  Proof. solve_contractive. Qed.
-  Definition lty_rec (C : lty Σ → lty Σ) `{!Contractive C} : lty Σ :=
-    fixpoint (lty_rec_aux C).
-Definition lty_forall {k} (C : kind_interp k Σ → lty Σ) : lty Σ := Lty (λ w,
-    ∀ A : kind_interp k Σ, WP w #() {{ C A }})%I.
-  Definition lty_exist {k} (C : kind_interp k Σ → lty Σ) : lty Σ := Lty (λ w,
-    ∃ A : kind_interp k Σ, ▷ C A w)%I.
-  Definition lty_ref_mut (A : lty Σ) : lty Σ := Lty (λ w,
-    ∃ (l : loc) (v : val), ⌜w = #l⌝ ∗ l ↦ v ∗ ▷ A v)%I.
-  Definition ref_shrN := nroot .@ "shr_ref".
-  Definition lty_ref_shr (A : lty Σ) : lty Σ := Lty (λ w,
-    ∃ l : loc, ⌜w = #l⌝ ∗ inv (ref_shrN .@ l) (∃ v, l ↦ v ∗ A v))%I.
-  Definition lty_mutex `{lockG Σ} (A : lty Σ) : lty Σ := Lty (λ w,
-    ∃ (γ : gname) (l : loc) (lk : val),
-      ⌜ w = PairV lk #l ⌝ ∗
-      is_lock γ lk (∃ v_inner, l ↦ v_inner ∗ A v_inner))%I.
-  Definition lty_mutexguard `{lockG Σ} (A : lty Σ) : lty Σ := Lty (λ w,
-    ∃ (γ : gname) (l : loc) (lk : val) (v : val),
-      ⌜ w = PairV lk #l ⌝ ∗
-      is_lock γ lk (∃ v_inner, l ↦ v_inner ∗ A v_inner) ∗
-      locked γ ∗ l ↦ v)%I.
-  Definition lty_chan `{chanG Σ} (P : lsty Σ) : lty Σ := Lty (λ w, w ↣ P)%I.
-End types.
-
-Notation "()" := lty_unit : kind_scope.
-Notation "'copy' A" := (lty_copy A) (at level 10) : kind_scope.
-Notation "'copy-' A" := (lty_copyminus A) (at level 10) : kind_scope.
-Notation "A → B" := (lty_copy (lty_arr A B)) : kind_scope.
-Notation "A ⊸ B" := (lty_arr A B) (at level 99, B at level 200, right associativity) : kind_scope.
-Infix "*" := lty_prod : kind_scope.
-Infix "+" := lty_sum : kind_scope.
-Notation any := lty_any.
-Notation "∀ A1 .. An , C" :=
-  (lty_forall (λ A1, .. (lty_forall (λ An, C%kind)) ..)) : kind_scope.
-Notation "∃ A1 .. An , C" :=
-  (lty_exist (λ A1, .. (lty_exist (λ An, C%kind)) ..)) : kind_scope.
-Notation "'ref_mut' A" := (lty_ref_mut A) (at level 10) : kind_scope.
-Notation "'ref_shr' A" := (lty_ref_shr A) (at level 10) : kind_scope.
-
-Notation "'mutex' A" := (lty_mutex A) (at level 10) : kind_scope.
-Notation "'mutexguard' A" := (lty_mutexguard A) (at level 10) : kind_scope.
-Notation "'chan' A" := (lty_chan A) (at level 10) : kind_scope.
+From iris.heap_lang Require Import metatheory.
+From iris.heap_lang.lib Require Export spawn par assert.
+From actris.logrel Require Export subtyping typing_judgment session_types.
+From actris.logrel Require Import environments.
+From actris.utils Require Import switch.
+From actris.channel Require Import proofmode.
 
 Section properties.
   Context `{heapG Σ}.
-  Implicit Types Γ : gmap string (lty Σ).
+  Implicit Types A B : ltty Σ.
+  Implicit Types S T : lsty Σ.
+  Implicit Types Γ : gmap string (ltty Σ).
+
+  (** Variable properties *)
+  Lemma ltyped_var Γ (x : string) A :
+    Γ !! x = Some A → ⊢ Γ ⊨ x : A ⫤ delete x Γ.
+  Proof.
+    iIntros (HΓx) "!>"; iIntros (vs) "HΓ /=".
+    iDestruct (env_ltyped_lookup with "HΓ") as (v ->) "[HA HΓ]"; first done.
+    iApply wp_value. eauto with iFrame.
+  Qed.
+
+  (** Subtyping *)
+  Theorem ltyped_subsumption Γ Γ2 e τ1 τ2 :
+    τ1 <: τ2 -∗ (Γ ⊨ e : τ1 ⫤ Γ2) -∗ (Γ ⊨ e : τ2 ⫤ Γ2).
+  Proof.
+    iIntros "#Hle #Hltyped" (vs) "!> Henv".
+    iDestruct ("Hltyped" with "Henv") as "Hltyped'".
+    iApply (wp_wand with "Hltyped' [Hle]").
+    iIntros (v) "[H1 $]". by iApply "Hle".
+  Qed.
 
   (** Basic properties *)
-  Global Instance lty_unit_unboxed : @LTyUnboxed Σ ().
-  Proof. by iIntros (v ->). Qed.
-  Global Instance lty_bool_unboxed : @LTyUnboxed Σ lty_bool.
-  Proof. iIntros (v). by iDestruct 1 as (b) "->". Qed.
-  Global Instance lty_int_unboxed : @LTyUnboxed Σ lty_int.
-  Proof. iIntros (v). by iDestruct 1 as (i) "->". Qed.
-
   Lemma ltyped_unit Γ : ⊢ Γ ⊨ #() : ().
   Proof. iIntros "!>" (vs) "Henv /=". iApply wp_value. eauto. Qed.
   Lemma ltyped_bool Γ (b : bool) : ⊢ Γ ⊨ #b : lty_bool.
@@ -89,76 +41,7 @@ Section properties.
   Lemma ltyped_nat Γ (n : Z) : ⊢ Γ ⊨ #n : lty_int.
   Proof. iIntros "!>" (vs) "Henv /=". iApply wp_value. eauto. Qed.
 
-  (** Operator Properties *)
-  Global Instance lty_bin_op_eq A : LTyUnboxed A → @LTyBinOp Σ EqOp A A lty_bool.
-  Proof.
-    iIntros (Q v1 v2) "A1 _". rewrite /bin_op_eval /lty_car /=.
-    iDestruct (lty_unboxed with "A1") as %Hunb.
-    rewrite decide_True; last solve_vals_compare_safe.
-    eauto.
-  Qed.
-  Global Instance lty_bin_op_arith op :
-    TCElemOf op [PlusOp; MinusOp; MultOp; QuotOp; RemOp;
-                 AndOp; OrOp; XorOp; ShiftLOp; ShiftROp] →
-    @LTyBinOp Σ op lty_int lty_int lty_int.
-  Proof.
-    iIntros (? v1 v2); iDestruct 1 as (i1) "->"; iDestruct 1 as (i2) "->".
-    repeat match goal with H : TCElemOf _ _ |- _ => inversion_clear H end;
-      rewrite /lty_car /=; eauto.
-  Qed.
-  Global Instance lty_bin_op_compare op :
-    TCElemOf op [LeOp; LtOp] →
-    @LTyBinOp Σ op lty_int lty_int lty_bool.
-  Proof.
-    iIntros (? v1 v2); iDestruct 1 as (i1) "->"; iDestruct 1 as (i2) "->".
-    repeat match goal with H : TCElemOf _ _ |- _ => inversion_clear H end;
-      rewrite /lty_car /=; eauto.
-  Qed.
-  Global Instance lty_bin_op_bool op :
-    TCElemOf op [AndOp; OrOp; XorOp] →
-    @LTyBinOp Σ op lty_bool lty_bool lty_bool.
-  Proof.
-    iIntros (? v1 v2); iDestruct 1 as (i1) "->"; iDestruct 1 as (i2) "->".
-    repeat match goal with H : TCElemOf _ _ |- _ => inversion_clear H end;
-      rewrite /lty_car /=; eauto.
-  Qed.
-
-  (** Variable properties *)
-  Lemma ltyped_var Γ (x : string) A :
-    Γ !! x = Some A → ⊢ Γ ⊨ x : A ⫤ delete x Γ.
-  Proof.
-    iIntros (HΓx) "!>".
-    iIntros (vs) "HΓ /=".
-    iDestruct (env_ltyped_lookup with "HΓ") as (v ->) "[HA HΓ]"; first done.
-    iApply wp_value. eauto with iFrame.
-  Qed.
-
-  (** Copy properties *)
-  Global Instance lty_copy_ne : NonExpansive (@lty_copy Σ).
-  Proof. solve_proper. Qed.
-
   (** Arrow properties *)
-  Global Instance lty_arr_contractive n :
-    Proper (dist_later n ==> dist_later n ==> dist n) lty_arr.
-  Proof.
-    intros A A' ? B B' ?.
-    apply lty_ne.
-    intros f.
-    f_equiv.
-    intros w.
-    f_equiv.
-    - by f_contractive.
-    - apply wp_contractive.
-      { apply _. }
-      intros q.
-      destruct n as [|n'].
-      + done.
-      + by simpl.
-  Qed.
-
-  Global Instance lty_arr_ne : NonExpansive2 (@lty_arr Σ _).
-  Proof. solve_proper. Qed.
-
   Lemma ltyped_app Γ1 Γ2 Γ3 e1 e2 A1 A2 :
     (Γ2 ⊨ e1 : A1 ⊸ A2 ⫤ Γ3) -∗ (Γ1 ⊨ e2 : A1 ⫤ Γ2) -∗
     Γ1 ⊨ e1 e2 : A2 ⫤ Γ3.
@@ -179,28 +62,53 @@ Section properties.
     iIntros (v) "HA1". wp_pures.
     iDestruct ("He" $!((binder_insert x v vs)) with "[HA1 HΓ]") as "He'".
     { iApply (env_ltyped_insert with "[HA1 //] HΓ"). }
-    iDestruct (wp_wand _ _ _ _ (λ v, A2 v) with "He' []") as "He'".
+    iDestruct (wp_wand _ _ _ _ (ltty_car A2) with "He' []") as "He'".
     { iIntros (w) "[$ _]". }
     destruct x as [|x]; rewrite /= -?subst_map_insert //.
+  Qed.
+
+  (* Typing rule for introducing copyable functions *)
+  Lemma ltyped_rec Γ Γ' f x e A1 A2 :
+    env_copy Γ Γ' -∗
+    (binder_insert f (A1 → A2)%lty (binder_insert x A1 Γ') ⊨ e : A2) -∗
+    Γ ⊨ (rec: f x := e) : A1 → A2 ⫤ ∅.
+  Proof.
+    iIntros "#Hcopy #He". iIntros (vs) "!> HΓ /=". iApply wp_fupd. wp_pures.
+    iDestruct ("Hcopy" with "HΓ") as "HΓ".
+    iMod (fupd_mask_mono with "HΓ") as "#HΓ"; first done.
+    iModIntro. iSplitL; last by iApply env_ltyped_empty.
+    iLöb as "IH".
+    iIntros (v) "!> HA1". wp_pures. set (r := RecV f x _).
+    iDestruct ("He" $!(binder_insert f r (binder_insert x v vs))
+                  with "[HΓ HA1]") as "He'".
+    { iApply (env_ltyped_insert with "IH").
+      iApply (env_ltyped_insert with "HA1 HΓ"). }
+    iDestruct (wp_wand _ _ _ _ (ltty_car A2) with "He' []") as "He'".
+    { iIntros (w) "[$ _]". }
+    destruct x as [|x], f as [|f]; rewrite /= -?subst_map_insert //.
+    destruct (decide (x = f)) as [->|].
+    - by rewrite subst_subst delete_idemp !insert_insert -subst_map_insert.
+    - rewrite subst_subst_ne // -subst_map_insert.
+      by rewrite -delete_insert_ne // -subst_map_insert.
   Qed.
 
   Lemma ltyped_let Γ1 Γ2 Γ3 (x : binder) e1 e2 A1 A2 :
     (Γ1 ⊨ e1 : A1 ⫤ Γ2) -∗ (binder_insert x A1 Γ2 ⊨ e2 : A2 ⫤ Γ3) -∗
     Γ1 ⊨ (let: x:=e1 in e2) : A2 ⫤ ∅.
-  Proof. iIntros "#He1 #He2". iApply ltyped_app=> //. by iApply ltyped_lam. Qed.
+  Proof. iIntros "#He1 #He2". iApply ltyped_app; last done. by iApply ltyped_lam. Qed.
 
-  Fixpoint lty_arr_list (As : list (lty Σ)) (B : lty Σ) : lty Σ :=
+  Fixpoint lty_arr_list (As : list (ltty Σ)) (B : ltty Σ) : ltty Σ :=
     match As with
     | [] => B
     | A :: As => A ⊸ lty_arr_list As B
     end.
 
   Lemma lty_arr_list_spec_step A As (e : expr) B ws y i :
-    (∀ v, lty_car A v -∗
-          WP subst_map (<[ y +:+ pretty i := v ]>ws)
-             (switch_lams y (S i) (length As) e) {{ lty_arr_list As B }}) -∗
-    WP subst_map ws (switch_lams y i (length (A::As)) e)
-       {{ lty_arr_list (A::As) B }}.
+    (∀ v, ltty_car A v -∗
+      WP subst_map (<[y+:+pretty i:=v]> ws)
+         (switch_lams y (S i) (length As) e) {{ ltty_car (lty_arr_list As B) }}) -∗
+    WP subst_map ws (switch_lams y i (S (length As)) e)
+       {{ ltty_car (lty_arr_list (A :: As) B) }}.
   Proof.
     iIntros "H". wp_pures. iIntros (v) "HA".
     iDestruct ("H" with "HA") as "H".
@@ -210,34 +118,25 @@ Section properties.
 
   Lemma lty_arr_list_spec As (e : expr) B ws y i n :
     n = length As →
-    (∀ vs, ([∗ list] A;v ∈ As;vs, (lty_car A) v) -∗
-           WP subst_map (map_string_seq y i vs ∪ ws) e {{ lty_car B }}) -∗
-    WP subst_map ws (switch_lams y i n e) {{ lty_arr_list As B }}.
+    (∀ vs, ([∗ list] A;v ∈ As;vs, ltty_car A v) -∗
+           WP subst_map (map_string_seq y i vs ∪ ws) e {{ ltty_car B }}) -∗
+    WP subst_map ws (switch_lams y i n e) {{ ltty_car (lty_arr_list As B) }}.
   Proof.
-    iIntros (Hlen) "H". iRevert (Hlen).
-    iInduction As as [|A As] "IH" forall (ws i e n)=> /=.
-    - iIntros (->).
-      iDestruct ("H" $! [] with "[$]") as "H"=> /=.
+    iIntros (Hlen) "H".
+    iInduction As as [|A As] "IH" forall (ws i e n Hlen); simplify_eq/=.
+    - iDestruct ("H" $! [] with "[$]") as "H"=> /=.
       by rewrite left_id_L.
-    - iIntros (->). iApply lty_arr_list_spec_step.
-      iIntros (v) "HA".
-      iApply ("IH" with "[H HA]")=> //.
-      iIntros (vs) "HAs".
-      iSpecialize ("H" $!(v::vs))=> /=.
+    - iApply lty_arr_list_spec_step. iIntros (v) "HA".
+      iApply ("IH" with "[//]"). iIntros (vs) "HAs".
+      iSpecialize ("H" $! (v::vs)); simpl.
       do 2 rewrite insert_union_singleton_l.
       rewrite (map_union_comm ({[y +:+ pretty i := v]})); last first.
       { apply map_disjoint_singleton_l_2.
         apply lookup_map_string_seq_None_lt. eauto. }
-      rewrite assoc_L. iApply ("H" with "[HA HAs]"). iFrame "HA HAs".
+      rewrite assoc_L. iApply ("H" with "[$HA $HAs]").
   Qed.
 
   (** Product properties  *)
-  Global Instance lty_prod_contractive n:
-    Proper (dist_later n ==> dist_later n ==> dist n) (@lty_prod Σ).
-  Proof. solve_contractive. Qed.
-  Global Instance lty_prod_ne : NonExpansive2 (@lty_prod Σ).
-  Proof. solve_proper. Qed.
-
   Lemma ltyped_pair Γ1 Γ2 Γ3 e1 e2 A1 A2 :
     (Γ2 ⊨ e1 : A1 ⫤ Γ3) -∗ (Γ1 ⊨ e2 : A2 ⫤ Γ2) -∗
     Γ1 ⊨ (e1,e2) : A1 * A2 ⫤ Γ3.
@@ -264,12 +163,6 @@ Section properties.
   Qed.
 
   (** Sum Properties *)
-  Global Instance lty_sum_contractive n :
-    Proper (dist_later n ==> dist_later n ==> dist n) (@lty_sum Σ).
-  Proof. solve_contractive. Qed.
-  Global Instance lty_sum_ne : NonExpansive2 (@lty_sum Σ).
-  Proof. solve_proper. Qed.
-
   Lemma ltyped_injl Γ e A1 A2 :
     (Γ ⊨ e : A1) -∗ Γ ⊨ InjL e : A1 + A2.
   Proof.
@@ -309,60 +202,42 @@ Section properties.
   Qed.
 
   (** Universal Properties *)
-  Global Instance lty_forall_ne k n :
-    Proper (pointwise_relation _ (dist n) ==> dist n) (@lty_forall Σ _ k).
-  Proof. solve_proper. Qed.
-  Global Instance lty_forall_contractive k n :
-    Proper (pointwise_relation _ (dist_later n) ==> dist n) (@lty_forall Σ _ k).
-  Proof.
-    intros F F' A. apply lty_ne=> w. f_equiv=> B.
-    apply (wp_contractive _ _ _ _ _)=> u. specialize (A B).
-    by destruct n as [|n]; simpl.
-  Qed.
-
-  Lemma ltyped_tlam Γ e k (C : kind_interp k Σ → lty Σ) :
-    (∀ A, Γ ⊨ e : C A ⫤ ∅) -∗ Γ ⊨ (λ: <>, e) : ∀ A, C A ⫤ ∅.
+  Lemma ltyped_tlam Γ e k (C : lty Σ k → ltty Σ) :
+    (∀ M, Γ ⊨ e : C M ⫤ ∅) -∗ Γ ⊨ (λ: <>, e) : ∀ M, C M ⫤ ∅.
   Proof.
     iIntros "#He" (vs) "!> HΓ /=". wp_pures.
     iSplitL; last by iApply env_ltyped_empty.
-    iIntros (A) "/=". wp_pures.
+    iIntros (M) "/=". wp_pures.
     iApply (wp_wand with "(He HΓ)"). iIntros (v) "[$ _]".
   Qed.
 
-  Lemma ltyped_tapp Γ Γ2 e k (C : kind_interp k Σ → lty Σ) A :
-    (Γ ⊨ e : ∀ A, C A ⫤ Γ2) -∗ Γ ⊨ e #() : C A ⫤ Γ2.
+  Lemma ltyped_tapp Γ Γ2 e k (C : lty Σ k → ltty Σ) M :
+    (Γ ⊨ e : ∀ M, C M ⫤ Γ2) -∗ Γ ⊨ e #() : C M ⫤ Γ2.
   Proof.
     iIntros "#He" (vs) "!> HΓ /=".
-    wp_apply (wp_wand with "(He [HΓ //])"); iIntros (w) "[HB HΓ]".
-    by iApply (wp_wand with "HB [HΓ]"); iIntros (v) "$ //".
+    wp_apply (wp_wand with "(He [HΓ //])"); iIntros (w) "[HB HΓ] /=".
+    iApply (wp_wand with "HB [HΓ]"). by iIntros (v) "$".
   Qed.
 
   (** Existential properties *)
-  Global Instance lty_exist_ne k n :
-    Proper (pointwise_relation _ (dist n) ==> dist n) (@lty_exist Σ k).
-  Proof. solve_proper. Qed.
-  Global Instance lty_exist_contractive k n :
-    Proper (pointwise_relation _ (dist_later n) ==> dist n) (@lty_exist Σ k).
-  Proof. solve_contractive. Qed.
-
-  Lemma ltyped_pack Γ e k (C : kind_interp k Σ → lty Σ) A :
-    (Γ ⊨ e : C A) -∗ Γ ⊨ e : ∃ A, C A.
+  Lemma ltyped_pack Γ e k (C : lty Σ k → ltty Σ) M :
+    (Γ ⊨ e : C M) -∗ Γ ⊨ e : ∃ M, C M.
   Proof.
     iIntros "#He" (vs) "!> HΓ /=".
-    wp_apply (wp_wand with "(He [HΓ //])"); iIntros (w) "[HB $]". by iExists A.
+    wp_apply (wp_wand with "(He [HΓ //])"); iIntros (w) "[HB $]". by iExists M.
   Qed.
 
   Definition unpack : val := λ: "exist" "f", "f" #() "exist".
 
-  Lemma ltyped_unpack k (C : kind_interp k Σ → lty Σ) B :
-    ⊢ ∅ ⊨ unpack : (∃ A, C A) → (∀ A, C A ⊸ B) ⊸ B.
+  Lemma ltyped_unpack k (C : lty Σ k → ltty Σ) B :
+    ⊢ ∅ ⊨ unpack : (∃ M, C M) → (∀ M, C M ⊸ B) ⊸ B.
   Proof.
     iIntros (vs) "!> HΓ /=". iApply wp_value.
     iSplitL; last by iApply env_ltyped_empty.
-    iIntros "!>" (v). iDestruct 1 as (A) "Hv".
+    iIntros "!>" (v). iDestruct 1 as (M) "Hv".
     rewrite /unpack. wp_pures.
     iIntros (fty) "Hfty". wp_pures.
-    iSpecialize ("Hfty" $! A).
+    iSpecialize ("Hfty" $! M).
     wp_bind (fty _). wp_apply (wp_wand with "Hfty").
     iIntros (f) "Hf".
     wp_apply (wp_wand with "(Hf [Hv //])").
@@ -370,13 +245,6 @@ Section properties.
   Qed.
 
   (** Mutable Reference properties *)
-  Global Instance lty_ref_mut_contractive : Contractive (@lty_ref_mut Σ _).
-  Proof. solve_contractive. Qed.
-  Global Instance lty_ref_mut_ne : NonExpansive2 (@lty_ref_mut Σ _).
-  Proof. solve_proper. Qed.
-  Global Instance lty_ref_mut_unboxed A : LTyUnboxed (ref_mut A).
-  Proof. iIntros (v). by iDestruct 1 as (i w ->) "?". Qed.
-
   Definition alloc : val := λ: "init", ref "init".
   Lemma ltyped_alloc A :
     ⊢ ∅ ⊨ alloc : A → ref_mut A.
@@ -436,13 +304,6 @@ Section properties.
   Qed.
 
   (** Weak Reference properties *)
-  Global Instance lty_ref_shr_contractive : Contractive (@lty_ref_shr Σ _).
-  Proof. solve_contractive. Qed.
-  Global Instance lty_ref_shr_ne : NonExpansive2 (@lty_ref_shr Σ _).
-  Proof. solve_proper. Qed.
-  Global Instance lty_ref_shr_unboxed A : LTyUnboxed (ref_shr A).
-  Proof. iIntros (v). by iDestruct 1 as (l ->) "?". Qed.
-
   Definition fetch_and_add : val := λ: "r" "inc", FAA "r" "inc".
   Lemma ltyped_fetch_and_add :
     ⊢ ∅ ⊨ fetch_and_add : ref_shr lty_int → lty_int → lty_int.
@@ -458,7 +319,7 @@ Section properties.
     iInv (ref_shrN .@ l) as (n) "[>Hl >Hn]" "Hclose".
     iDestruct "Hn" as %[m ->]. wp_faa.
     iMod ("Hclose" with "[Hl]") as %_.
-    { iExists #(m + k). iFrame "Hl". by iExists (m + k). }
+    { iExists #(m + k). iFrame "Hl". by iExists (m + k)%Z. }
     by iExists m.
   Qed.
 
@@ -484,7 +345,7 @@ Section properties.
   (*   by iFrame "Hr". *)
   (* Qed. *)
 
-  Lemma ltyped_ref_shrstore (A : lty Σ) :
+  Lemma ltyped_ref_shrstore A :
     ⊢ ∅ ⊨ store : ref_shr A → A → ref_shr A.
   Proof.
     iIntros (vs) "!> _ /=". iApply wp_value.
@@ -504,16 +365,6 @@ Section properties.
     Context `{lockG Σ}.
 
     (** Mutex properties *)
-    Global Instance lty_mutex_contractive : Contractive (@lty_mutex Σ _ _).
-    Proof. solve_contractive. Qed.
-    Global Instance lty_mutex_ne : NonExpansive (@lty_mutex Σ _ _).
-    Proof. solve_proper. Qed.
-
-    Global Instance lty_mutexguard_contractive : Contractive (@lty_mutexguard Σ _ _).
-    Proof. solve_contractive. Qed.
-    Global Instance lty_mutexguard_ne : NonExpansive (@lty_mutexguard Σ _ _).
-    Proof. solve_proper. Qed.
-
     Definition mutexalloc : val := λ: "x", (newlock #(), ref "x").
     Lemma ltyped_mutexalloc A :
       ⊢ ∅ ⊨ mutexalloc : A → mutex A.
@@ -524,7 +375,7 @@ Section properties.
       wp_alloc l as "Hl".
       wp_bind (newlock _).
       set (N := nroot .@ "makelock").
-      iAssert (∃ inner, l ↦ inner ∗ A inner)%I with "[Hl Hv]" as "Hlock".
+      iAssert (∃ inner, l ↦ inner ∗ ltty_car A inner)%I with "[Hl Hv]" as "Hlock".
       { iExists v. iFrame "Hl Hv". }
       wp_apply (newlock_spec with "Hlock").
       iIntros (lk γ) "Hlock".
@@ -563,11 +414,11 @@ Section properties.
       iIntros (w2) "Hw2". wp_pures.
       iDestruct "Hw2" as (γ l lk inner ->) "[#Hlock [Hlocked Hinner]]".
       wp_store.
-      iAssert (∃ inner : val, l ↦ inner ∗ A inner)%I
+      iAssert (∃ inner : val, l ↦ inner ∗ ltty_car A inner)%I
         with "[Hinner Hw1]" as "Hinner".
       { iExists w1. iFrame "Hinner Hw1". }
       wp_bind (release _).
-      wp_apply (release_spec γ _ (∃ inner, l ↦ inner ∗ A inner)%I
+      wp_apply (release_spec γ _ (∃ inner, l ↦ inner ∗ ltty_car A inner)%I
                   with "[Hlocked Hinner]").
       { iFrame "Hlock Hlocked".
         iDestruct "Hinner" as (v) "[Hl HA]". eauto with iFrame. }
@@ -589,7 +440,7 @@ Section properties.
       iSplitL; last by iApply env_ltyped_empty.
       iIntros "!>" (fa) "Hfa". rewrite /parallel. wp_pures.
       iIntros (fb) "Hfb". wp_pures.
-      wp_apply (par_spec A B with "[Hfa] [Hfb]").
+      wp_apply (par_spec (ltty_car A) (ltty_car B) with "[Hfa] [Hfb]").
       - by wp_apply "Hfa".
       - by wp_apply "Hfb".
       - iIntros (v1 v2) "[HA HB] !>". iExists v1, v2. eauto with iFrame.
@@ -599,12 +450,9 @@ Section properties.
   Section with_chan.
     Context `{chanG Σ}.
 
-    Global Instance lty_chan_ne : NonExpansive lty_chan.
-    Proof. solve_proper. Qed.
-
     Definition chanalloc : val := λ: "u", let: "cc" := new_chan #() in "cc".
     Lemma ltyped_chanalloc S :
-      ⊢ ∅ ⊨ chanalloc : () → (chan S * chan (lsty_dual S)).
+      ⊢ ∅ ⊨ chanalloc : () → (chan S * chan (lty_dual S)).
     Proof.
       iIntros (vs) "!> HΓ /=". iApply wp_value.
       iSplitL; last by iApply env_ltyped_empty.
@@ -626,8 +474,8 @@ Section properties.
     Qed.
 
     Lemma ltyped_send Γ Γ' (x : string) e A S :
-      (Γ ⊨ e : A ⫤ <[x:=(chan (<!!> A; S))%kind]> Γ') -∗
-      Γ ⊨ send x e : () ⫤ <[x:=(chan S)%kind]> Γ'.
+      (Γ ⊨ e : A ⫤ <[x:=(chan (<!!> A; S))%lty]> Γ') -∗
+      Γ ⊨ send x e : () ⫤ <[x:=(chan S)%lty]> Γ'.
     Proof.
       iIntros "#He !>" (vs) "HΓ"=> /=.
       wp_bind (subst_map vs e).
@@ -654,7 +502,7 @@ Section properties.
     Qed.
 
     Lemma ltyped_recv Γ (x : string) A S :
-      ⊢ <[x := (chan (<??> A; S))%kind]> Γ ⊨ recv x : A ⫤ <[x:=(chan S)%kind]> Γ.
+      ⊢ <[x := (chan (<??> A; S))%lty]> Γ ⊨ recv x : A ⫤ <[x:=(chan S)%lty]> Γ.
     Proof.
       iIntros "!>" (vs) "HΓ"=> /=.
       iDestruct (env_ltyped_lookup with "HΓ") as (v' Heq) "[Hc HΓ]".
@@ -669,7 +517,7 @@ Section properties.
     Definition chanselect : val := λ: "c" "i", send "c" "i";; "c".
     Lemma ltyped_chanselect Γ (c : val) (i : Z) S Ss :
       Ss !! i = Some S →
-      (Γ ⊨ c : chan (lsty_select Ss)) -∗
+      (Γ ⊨ c : chan (lty_select Ss)) -∗
       Γ ⊨ chanselect c #i : chan S.
     Proof.
       iIntros (Hin) "#Hc !>".
@@ -688,8 +536,8 @@ Section properties.
 
     Lemma ltyped_chanbranch Ss A xs :
       (∀ x, x ∈ xs ↔ is_Some (Ss !! x)) →
-      ⊢ ∅ ⊨ chanbranch xs : chan (lsty_branch Ss) ⊸
-        lty_arr_list ((λ x, (chan (Ss !!! x) ⊸ A)%kind) <$> xs) A.
+      ⊢ ∅ ⊨ chanbranch xs : chan (lty_branch Ss) ⊸
+        lty_arr_list ((λ x, (chan (Ss !!! x) ⊸ A)%lty) <$> xs) A.
     Proof.
       iIntros (Hdom) "!>". iIntros (vs) "Hvs".
       iApply wp_value.
