theories/channel/proto.v
@@ -25,9 +25,10 @@ specifications of the message-passing primitives are defined in terms of the
 protocol connectives. *)
 From iris.algebra Require Import excl_auth.
 From iris.bi Require Import telescopes.
-From iris.program_logic Require Import language.
 From iris.proofmode Require Import tactics.
+From iris.base_logic Require Export lib.iprop.
 From iris.base_logic Require Import lib.own.
+From iris.program_logic Require Import language.
 From actris.channel Require Import proto_model.
 Set Default Proof Using "Type".
 Export action.
