theories/logrel/environments.v
@@ -1,0 +1,162 @@
+From actris.logrel Require Export term_types.
+From iris.proofmode Require Import tactics.
+
+Definition env_ltyped {Σ} (Γ : gmap string (ltty Σ))
+    (vs : gmap string val) : iProp Σ :=
+  ([∗ map] i ↦ A ∈ Γ, ∃ v, ⌜vs !! i = Some v⌝ ∗ ltty_car A v)%I.
+
+Definition env_split {Σ} (Γ Γ1 Γ2 : gmap string (ltty Σ)) : iProp Σ :=
+  (■ ∀ vs, env_ltyped Γ vs ∗-∗ (env_ltyped Γ1 vs ∗ env_ltyped Γ2 vs))%I.
+
+Definition env_copy {Σ} (Γ Γ' : gmap string (ltty Σ)) : iProp Σ :=
+  (■ ∀ vs, env_ltyped Γ vs -∗ □ env_ltyped Γ' vs)%I.
+
+Section env.
+  Context {Σ : gFunctors}.
+  Implicit Types A : ltty Σ.
+  Implicit Types Γ : gmap string (ltty Σ).
+
+  Lemma env_ltyped_empty vs : ⊢@{iPropI Σ} env_ltyped ∅ vs.
+  Proof. by iApply big_sepM_empty. Qed.
+
+  Lemma env_ltyped_lookup Γ vs x A :
+    Γ !! x = Some A →
+    env_ltyped Γ vs -∗
+    ∃ v, ⌜ vs !! x = Some v ⌝ ∗ ltty_car A v ∗ env_ltyped (delete x Γ) vs.
+  Proof.
+    iIntros (HΓx) "HΓ".
+    iPoseProof (big_sepM_delete with "HΓ") as "[HA H]"; eauto.
+    iDestruct "HA" as (v) "HA"; eauto with iFrame.
+  Qed.
+
+  Lemma env_ltyped_insert Γ vs x A v :
+    ltty_car A v -∗
+    env_ltyped Γ vs -∗
+    env_ltyped (binder_insert x A Γ) (binder_insert x v vs).
+  Proof.
+    destruct x as [|x]=> /=; first by auto.
+    iIntros "HA HΓ".
+    rewrite /env_ltyped.
+    set Γ' := <[x:=A]> Γ.
+    assert (Hx: Γ' !! x = Some A).
+    { apply lookup_insert. }
+    iApply (big_sepM_delete _ _ _ _ Hx).
+    iSplitL "HA".
+    { iExists v. rewrite lookup_insert. auto. }
+    assert (Hsub: delete x Γ' ⊆ Γ).
+    { rewrite delete_insert_delete. apply delete_subseteq. }
+    iPoseProof (big_sepM_subseteq _ _ _ Hsub with "HΓ") as "HΓ".
+    iApply (big_sepM_mono with "HΓ"). simpl.
+    iIntros (y B Hy) "HB".
+    iDestruct "HB" as (w Hw) "HB".
+    iExists w. iFrame. iPureIntro.
+    apply lookup_delete_Some in Hy.
+    destruct Hy as [Hxy _].
+    by rewrite -Hw lookup_insert_ne.
+  Qed.
+
+  Lemma env_split_id_l Γ : ⊢ env_split Γ ∅ Γ.
+  Proof.
+    iIntros "!>" (vs).
+    iSplit; [iIntros "$" | iIntros "[_ $]"]; iApply env_ltyped_empty.
+  Qed.
+  Lemma env_split_id_r Γ : ⊢ env_split Γ Γ ∅.
+  Proof.
+    iIntros "!>" (vs).
+    iSplit; [iIntros "$" | iIntros "[$ _]"]; iApply env_ltyped_empty.
+  Qed.
+
+  Lemma env_split_empty : ⊢@{iPropI Σ} env_split ∅ ∅ ∅.
+  Proof.
+    iIntros "!>" (vs).
+    iSplit; [iIntros "HΓ" | iIntros "[HΓ1 HΓ2]"]; auto.
+  Qed.
+
+  (* TODO: Get rid of side condition that x does not appear in Γ1 *)
+  Lemma env_split_left Γ Γ1 Γ2 x A:
+    Γ !! x = None → Γ1 !! x = None →
+    env_split Γ Γ1 Γ2 -∗
+    env_split (<[x := A]> Γ) (<[x := A]> Γ1) Γ2.
+  Proof.
+    iIntros (HΓx HΓ2x) "#Hsplit !>". iIntros (vs).
+    iSplit.
+    - iIntros "HΓ".
+      iPoseProof (big_sepM_insert with "HΓ") as "[Hv HΓ]"; first by assumption.
+      iDestruct ("Hsplit" with "HΓ") as "[HΓ1 $]".
+      iApply (big_sepM_insert_2 with "[Hv]"); simpl; eauto.
+    - iIntros "[HΓ1 HΓ2]".
+      iPoseProof (big_sepM_insert with "HΓ1") as "[Hv HΓ1]"; first by assumption.
+      iApply (big_sepM_insert_2 with "[Hv]")=> //.
+      iApply "Hsplit". iFrame "HΓ1 HΓ2".
+  Qed.
+
+  Lemma env_split_comm Γ Γ1 Γ2:
+    env_split Γ Γ1 Γ2 -∗ env_split Γ Γ2 Γ1.
+  Proof.
+    iIntros "#Hsplit" (vs) "!>".
+    iSplit.
+    - iIntros "HΓ". by iDestruct ("Hsplit" with "HΓ") as "[$ $]".
+    - iIntros "[HΓ1 HΓ2]". iApply "Hsplit". iFrame.
+  Qed.
+
+  (* TODO: Get rid of side condition that x does not appear in Γ2 *)
+  Lemma env_split_right Γ Γ1 Γ2 x A:
+    Γ !! x = None → Γ2 !! x = None →
+    env_split Γ Γ1 Γ2 -∗
+    env_split (<[x := A]> Γ) Γ1 (<[x := A]> Γ2).
+  Proof.
+    iIntros (HΓx HΓ2x) "Hsplit".
+    iApply env_split_comm. iApply env_split_left=> //.
+    by iApply env_split_comm.
+  Qed.
+
+  (* TODO: Get rid of side condition that x does not appear in Γ *)
+  Lemma env_split_copyable Γ Γ1 Γ2 (x : string) A:
+    Γ !! x = None → Γ1 !! x = None → Γ2 !! x = None →
+    lty_copyable A -∗
+    env_split Γ Γ1 Γ2 -∗
+    env_split (<[x:=A]> Γ) (<[x:=A]> Γ1) (<[x:=A]> Γ2).
+  Proof.
+    iIntros (HΓx HΓ1x HΓ2x) "#Hcopy #Hsplit". iIntros (vs) "!>".
+    iSplit.
+    - iIntros "HΓ".
+      iPoseProof (big_sepM_insert with "HΓ") as "[Hv HΓ]"; first by assumption.
+      iDestruct "Hv" as (v ?) "HAv2".
+      iDestruct ("Hcopy" with "HAv2") as "#HAv".
+      iDestruct ("Hsplit" with "HΓ") as "[HΓ1 HΓ2]".
+      iSplitL "HΓ1"; iApply big_sepM_insert_2; simpl; eauto.
+    - iIntros "[HΓ1 HΓ2]".
+      iPoseProof (big_sepM_insert with "HΓ1") as "[Hv HΓ1]"; first by assumption.
+      iPoseProof (big_sepM_insert with "HΓ2") as "[_ HΓ2]"; first by assumption.
+      iApply (big_sepM_insert_2 with "[Hv]")=> //.
+      iApply "Hsplit". iFrame "HΓ1 HΓ2".
+  Qed.
+
+  Lemma env_copy_empty : ⊢@{iPropI Σ} env_copy ∅ ∅.
+  Proof. iIntros (vs) "!> _ !> ". by rewrite /env_ltyped. Qed.
+
+  Lemma env_copy_extend x A Γ Γ' :
+    Γ !! x = None →
+    env_copy Γ Γ' -∗
+    env_copy (<[x:=A]> Γ) Γ'.
+  Proof.
+    iIntros (HΓ) "#Hcopy". iIntros (vs) "!> Hvs". rewrite /env_ltyped.
+    iDestruct (big_sepM_insert with "Hvs") as "[_ Hvs]"; first by assumption.
+    iApply ("Hcopy" with "Hvs").
+  Qed.
+
+  Lemma env_copy_extend_copyable x A Γ Γ' :
+    Γ !! x = None →
+    Γ' !! x = None →
+    lty_copyable A -∗
+    env_copy Γ Γ' -∗
+    env_copy (<[x:=A]> Γ) (<[x:=A]> Γ').
+  Proof.
+    iIntros (HΓx HΓ'x) "#HcopyA #Hcopy". iIntros (vs) "!> Hvs". rewrite /env_ltyped.
+    iDestruct (big_sepM_insert with "Hvs") as "[HA Hvs]"; first done.
+    iDestruct ("Hcopy" with "Hvs") as "#Hvs'".
+    iDestruct "HA" as (v ?) "HA2".
+    iDestruct ("HcopyA" with "HA2") as "#HA".
+    iIntros "!>". iApply big_sepM_insert; first done. iSplitL; eauto.
+  Qed.
+End env.
