theories/logrel/operators.v
@@ -1,0 +1,71 @@
+From actris.logrel Require Export term_types.
+From iris.heap_lang Require Import proofmode.
+
+(** Semantic operator typing *)
+Class LTyUnboxed {Σ} (A : ltty Σ) :=
+  lty_unboxed v :
+    ltty_car A v -∗ ⌜ val_is_unboxed v ⌝.
+
+Class LTyUnOp {Σ} (op : un_op) (A B : ltty Σ) :=
+  lty_un_op v :
+    ltty_car A v -∗ ∃ w, ⌜ un_op_eval op v = Some w ⌝ ∧ ltty_car B w.
+
+Class LTyBinOp {Σ} (op : bin_op) (A1 A2 B : ltty Σ) :=
+  lty_bin_op v1 v2 :
+    ltty_car A1 v1 -∗ ltty_car A2 v2 -∗
+    ∃ w, ⌜ bin_op_eval op v1 v2 = Some w ⌝ ∧ ltty_car B w.
+
+Section operators.
+  Context {Σ : gFunctors}.
+  Implicit Types A B : ltty Σ.
+
+  (* Unboxed types *)
+  Global Instance lty_unit_unboxed : LTyUnboxed (Σ:=Σ) ().
+  Proof. by iIntros (v ->). Qed.
+  Global Instance lty_bool_unboxed : LTyUnboxed (Σ:=Σ) lty_bool.
+  Proof. iIntros (v). by iDestruct 1 as (b) "->". Qed.
+  Global Instance lty_int_unboxed : LTyUnboxed (Σ:=Σ) lty_int.
+  Proof. iIntros (v). by iDestruct 1 as (i) "->". Qed.
+  Global Instance lty_ref_mut_unboxed `{heapG Σ} A : LTyUnboxed (ref_mut A).
+  Proof. iIntros (v). by iDestruct 1 as (i w ->) "?". Qed.
+  Global Instance lty_ref_shr_unboxed `{heapG Σ} A : LTyUnboxed (ref_shr A).
+  Proof. iIntros (v). by iDestruct 1 as (l ->) "?". Qed.
+
+  (* Operator typing *)
+  Global Instance lty_un_op_int op : LTyUnOp (Σ:=Σ) op lty_int lty_int.
+  Proof. iIntros (?). iDestruct 1 as (i) "->". destruct op; eauto. Qed.
+  Global Instance lty_un_op_bool : LTyUnOp (Σ:=Σ) NegOp lty_bool lty_bool.
+  Proof. iIntros (?). iDestruct 1 as (i) "->". eauto. Qed.
+
+  Global Instance lty_bin_op_eq A : LTyUnboxed A → LTyBinOp EqOp A A lty_bool.
+  Proof.
+    iIntros (? v1 v2) "A1 _". rewrite /bin_op_eval /ltty_car /=.
+    iDestruct (lty_unboxed with "A1") as %Hunb.
+    rewrite decide_True; [eauto|solve_vals_compare_safe].
+  Qed.
+  Global Instance lty_bin_op_arith op :
+    TCElemOf op [PlusOp; MinusOp; MultOp; QuotOp; RemOp;
+                 AndOp; OrOp; XorOp; ShiftLOp; ShiftROp] →
+    LTyBinOp (Σ:=Σ) op lty_int lty_int lty_int.
+  Proof.
+    iIntros (? v1 v2); iDestruct 1 as (i1) "->"; iDestruct 1 as (i2) "->".
+    repeat match goal with H : TCElemOf _ _ |- _ => inversion_clear H end;
+      rewrite /ltty_car /=; eauto.
+  Qed.
+  Global Instance lty_bin_op_compare op :
+    TCElemOf op [LeOp; LtOp] →
+    LTyBinOp (Σ:=Σ) op lty_int lty_int lty_bool.
+  Proof.
+    iIntros (? v1 v2); iDestruct 1 as (i1) "->"; iDestruct 1 as (i2) "->".
+    repeat match goal with H : TCElemOf _ _ |- _ => inversion_clear H end;
+      rewrite /ltty_car /=; eauto.
+  Qed.
+  Global Instance lty_bin_op_bool op :
+    TCElemOf op [AndOp; OrOp; XorOp] →
+    LTyBinOp (Σ:=Σ) op lty_bool lty_bool lty_bool.
+  Proof.
+    iIntros (? v1 v2); iDestruct 1 as (i1) "->"; iDestruct 1 as (i2) "->".
+    repeat match goal with H : TCElemOf _ _ |- _ => inversion_clear H end;
+      rewrite /ltty_car /=; eauto.
+  Qed.
+End operators.
