theories/logrel/subtyping_rules.v
@@ -1,0 +1,433 @@
+From iris.bi.lib Require Import core.
+From iris.base_logic.lib Require Import invariants.
+From iris.proofmode Require Import tactics.
+From actris.logrel Require Export subtyping term_types session_types.
+
+Section subtyping_rules.
+  Context `{heapG Σ, chanG Σ}.
+  Implicit Types A : ltty Σ.
+  Implicit Types S : lsty Σ.
+
+  (** Generic rules *)
+  Lemma lty_le_refl {k} (M : lty Σ k) : ⊢ M <: M.
+  Proof.
+    destruct k.
+    - by iIntros (v) "!> H".
+    - iModIntro. iApply iProto_le_refl.
+  Qed.
+  Lemma lty_le_trans {k} (M1 M2 M3 : lty Σ k) : M1 <: M2 -∗ M2 <: M3 -∗ M1 <: M3.
+  Proof.
+    destruct k.
+    - iIntros "#H1 #H2" (v) "!> H". iApply "H2". by iApply "H1".
+    - iIntros "#H1 #H2 !>". by iApply iProto_le_trans.
+  Qed.
+
+  Lemma lty_bi_le_refl {k} (M : lty Σ k) : ⊢ M <:> M.
+  Proof. iSplit; iApply lty_le_refl. Qed.
+  Lemma lty_bi_le_trans {k} (M1 M2 M3 : lty Σ k) : M1 <:> M2 -∗ M2 <:> M3 -∗ M1 <:> M3.
+  Proof. iIntros "#[H11 H12] #[H21 H22]". iSplit; by iApply lty_le_trans. Qed.
+  Lemma lty_bi_le_sym {k} (M1 M2 : lty Σ k) : M1 <:> M2 -∗ M2 <:> M1.
+  Proof. iIntros "#[??]"; by iSplit. Qed.
+
+  Lemma lty_le_l {k} (M1 M2 M3 : lty Σ k) : M1 <:> M2 -∗ M2 <: M3 -∗ M1 <: M3.
+  Proof. iIntros "#[H1 _] #H2". by iApply lty_le_trans. Qed.
+  Lemma lty_le_r {k} (M1 M2 M3 : lty Σ k) : M1 <: M2 -∗ M2 <:> M3 -∗ M1 <: M3.
+  Proof. iIntros "#H1 #[H2 _]". by iApply lty_le_trans. Qed.
+
+  Lemma lty_le_rec_unfold {k} (C : lty Σ k → lty Σ k) `{!Contractive C} :
+    ⊢ lty_rec C <:> C (lty_rec C).
+  Proof.
+    iSplit.
+    - rewrite {1}/lty_rec fixpoint_unfold. iApply lty_le_refl.
+    - rewrite {2}/lty_rec fixpoint_unfold. iApply lty_le_refl.
+  Qed.
+
+  Lemma lty_le_rec {k} (C1 C2 : lty Σ k → lty Σ k) `{Contractive C1, Contractive C2} :
+    (∀ M1 M2, ▷ (M1 <: M2) -∗ C1 M1 <: C2 M2) -∗
+    lty_rec C1 <: lty_rec C2.
+  Proof.
+    iIntros "#Hle". iLöb as "IH".
+    iApply lty_le_l; [iApply lty_le_rec_unfold|].
+    iApply lty_le_r; [|iApply lty_bi_le_sym; iApply lty_le_rec_unfold].
+    by iApply "Hle".
+  Qed.
+
+  (** Term subtyping *)
+  Lemma lty_le_any A : ⊢ A <: any.
+  Proof. by iIntros (v) "!> H". Qed.
+  Lemma lty_copyable_any : ⊢@{iPropI Σ} lty_copyable any.
+  Proof. iIntros (v) "!> #Hv !>". iFrame "Hv". Qed.
+
+  Lemma lty_le_copy A B : A <: B -∗ copy A <: copy B.
+  Proof. iIntros "#Hle". iIntros (v) "!> #HA !>". by iApply "Hle". Qed.
+  Lemma lty_le_copy_elim A : ⊢ copy A <: A.
+  Proof. by iIntros (v) "!> #H". Qed.
+  Lemma lty_copyable_copy A : ⊢@{iPropI Σ} lty_copyable (copy A).
+  Proof. iIntros (v) "!> #Hv !>". iFrame "Hv". Qed.
+
+  Lemma lty_le_copy_inv A B : A <: B -∗ copy- A <: copy- B.
+  Proof.
+    iIntros "#Hle !>" (v) "#HA". iApply (coreP_wand (ltty_car A v) with "[] HA").
+    iIntros "{HA} !> !>". iApply "Hle".
+  Qed.
+  Lemma lty_le_copy_inv_intro A : ⊢ A <: copy- A.
+  Proof. iIntros "!>" (v). iApply coreP_intro. Qed.
+  Lemma lty_le_copy_inv_elim A : ⊢ copy- (copy A) <: A.
+  Proof. iIntros (v) "!> #H". iApply (coreP_elim with "H"). Qed.
+  Lemma lty_copyable_copy_inv A : ⊢ lty_copyable (copy- A).
+  Proof. iIntros (v) "!> #Hv !>". iFrame "Hv". Qed.
+
+  Lemma lty_copyable_unit : ⊢@{iPropI Σ} lty_copyable ().
+  Proof. iIntros (v) "!> #Hv !>". iFrame "Hv". Qed.
+  Lemma lty_copyable_bool : ⊢@{iPropI Σ} lty_copyable lty_bool.
+  Proof. iIntros (v) "!> #Hv !>". iFrame "Hv". Qed.
+  Lemma lty_copyable_int : ⊢@{iPropI Σ} lty_copyable lty_int.
+  Proof. iIntros (v) "!> #Hv !>". iFrame "Hv". Qed.
+
+  Lemma lty_le_arr A11 A12 A21 A22 :
+    ▷ (A21 <: A11) -∗ ▷ (A12 <: A22) -∗
+    (A11 ⊸ A12) <: (A21 ⊸ A22).
+  Proof.
+    iIntros "#H1 #H2" (v) "!> H". iIntros (w) "H'".
+    iApply (wp_step_fupd); first done.
+    { iIntros "!>!>!>". iExact "H2". }
+    iApply (wp_wand with "(H (H1 H'))"). iIntros (v') "H Hle !>".
+    by iApply "Hle".
+  Qed.
+  Lemma lty_le_arr_copy A11 A12 A21 A22 :
+    ▷ (A21 <: A11) -∗ ▷ (A12 <: A22) -∗
+    (A11 → A12) <: (A21 → A22).
+  Proof. iIntros "#H1 #H2" (v) "!> #H !>". by iApply lty_le_arr. Qed.
+
+  Lemma lty_le_prod A11 A12 A21 A22 :
+    ▷ (A11 <: A21) -∗ ▷ (A12 <: A22) -∗
+    A11 * A12 <: A21 * A22.
+  Proof.
+    iIntros "#H1 #H2" (v) "!>". iDestruct 1 as (w1 w2 ->) "[H1' H2']".
+    iExists _, _.
+    iDestruct ("H1" with "H1'") as "$".
+    by iDestruct ("H2" with "H2'") as "$".
+  Qed.
+  (* TODO(COPY): Show derived rules about copyability of products, sums, etc. *)
+  Lemma lty_le_prod_copy A B :
+    ⊢ copy A * copy B <:> copy (A * B).
+  Proof.
+    iSplit; iModIntro; iIntros (v) "#Hv"; iDestruct "Hv" as (v1 v2 ->) "[Hv1 Hv2]".
+    - iModIntro. iExists v1, v2. iSplit; [done|]. iSplitL; auto.
+    - iExists v1, v2. iSplit; [done|]. auto.
+  Qed.
+
+  Lemma lty_le_sum A11 A12 A21 A22 :
+    ▷ (A11 <: A21) -∗ ▷ (A12 <: A22) -∗
+    A11 + A12 <: A21 + A22.
+  Proof.
+    iIntros "#H1 #H2" (v) "!> [H | H]"; iDestruct "H" as (w ->) "H".
+    - iDestruct ("H1" with "H") as "H1'". iLeft; eauto.
+    - iDestruct ("H2" with "H") as "H2'". iRight; eauto.
+  Qed.
+  Lemma lty_le_sum_copy A B :
+    ⊢ copy A + copy B <:> copy (A + B).
+  Proof.
+    iSplit; iModIntro; iIntros (v);
+      iDestruct 1 as "#[Hv|Hv]"; iDestruct "Hv" as (w ?) "Hw";
+      try iModIntro; first [iLeft; by auto|iRight; by auto].
+  Qed.
+
+  Lemma lty_le_forall C1 C2 :
+    ▷ (∀ A, C1 A <: C2 A) -∗
+    (∀ A, C1 A) <: (∀ A, C2 A).
+  Proof.
+    iIntros "#Hle" (v) "!> H". iIntros (w).
+    iApply (wp_step_fupd); first done.
+    { iIntros "!>!>!>". iExact "Hle". }
+    iApply (wp_wand with "H"). iIntros (v') "H Hle' !>".
+    by iApply "Hle'".
+  Qed.
+  (* TODO(COPY) TODO(VALUERES): Do the forall type former, once we have the value restriction *)
+
+  Lemma lty_le_exist C1 C2 :
+    ▷ (∀ A, C1 A <: C2 A) -∗
+    (∃ A, C1 A) <: (∃ A, C2 A).
+  Proof.
+    iIntros "#Hle" (v) "!>". iDestruct 1 as (A) "H". iExists A. by iApply "Hle".
+  Qed.
+  Lemma lty_le_exist_elim C B :
+    ⊢ C B <: ∃ A, C A.
+  Proof. iIntros "!>" (v) "Hle". by iExists B. Qed.
+  Lemma lty_le_exist_copy F :
+    ⊢ (∃ A, copy (F A)) <:> copy (∃ A, F A).
+  Proof.
+    iSplit; iIntros "!>" (v); iDestruct 1 as (A) "#Hv";
+      iExists A; repeat iModIntro; iApply "Hv".
+  Qed.
+
+  (* TODO(COPY): Commuting rule for μ, allowing `copy` to move outside the μ *)
+  Lemma lty_rec_copy C `{!Contractive C} :
+    (∀ A, ▷ lty_copyable A -∗ lty_copyable (C A)) -∗ lty_copyable (lty_rec C).
+  Proof.
+    iIntros "#Hcopy".
+    iLöb as "IH".
+    iIntros (v) "!> Hv".
+    rewrite /lty_rec.
+    rewrite {2}fixpoint_unfold.
+    iSpecialize ("Hcopy" with "IH").
+    iSpecialize ("Hcopy" with "Hv").
+    iDestruct "Hcopy" as "#Hcopy".
+    iModIntro.
+    iEval (rewrite fixpoint_unfold).
+    iApply "Hcopy".
+  Qed.
+
+  Lemma lty_le_ref_mut A1 A2 :
+    ▷ (A1 <: A2) -∗
+    ref_mut A1 <: ref_mut A2.
+  Proof.
+    iIntros "#H1" (v) "!>". iDestruct 1 as (l w ->) "[Hl HA]".
+    iDestruct ("H1" with "HA") as "HA".
+    iExists l, w. by iFrame.
+  Qed.
+
+  Lemma lty_le_shr_ref A1 A2 :
+    ▷ (A1 <:> A2) -∗
+    ref_shr A1 <: ref_shr A2.
+  Proof.
+    iIntros "#[Hle1 Hle2]" (v) "!>". iDestruct 1 as (l ->) "Hinv".
+    iExists l. iSplit; first done.
+    iApply (inv_iff with "Hinv"). iIntros "!> !>". iSplit.
+    - iDestruct 1 as (v) "[Hl HA]". iExists v. iFrame "Hl". by iApply "Hle1".
+    - iDestruct 1 as (v) "[Hl HA]". iExists v. iFrame "Hl". by iApply "Hle2".
+  Qed.
+  Lemma lty_copyable_shr_ref A :
+    ⊢ lty_copyable (ref_shr A).
+  Proof. iIntros (v) "!> #Hv !>". iFrame "Hv". Qed.
+
+  Lemma lty_le_mutex A1 A2 :
+    ▷ (A1 <:> A2) -∗
+    mutex A1 <: mutex A2.
+  Proof.
+    iIntros "#[Hle1 Hle2]" (v) "!>". iDestruct 1 as (γ l lk ->) "Hinv".
+    iExists γ, l, lk. iSplit; first done.
+    iApply (spin_lock.is_lock_iff with "Hinv").
+    iIntros "!> !>". iSplit.
+    - iDestruct 1 as (v) "[Hl HA]". iExists v. iFrame "Hl". by iApply "Hle1".
+    - iDestruct 1 as (v) "[Hl HA]". iExists v. iFrame "Hl". by iApply "Hle2".
+  Qed.
+  Lemma lty_copyable_mutex A :
+    ⊢ lty_copyable (mutex A).
+  Proof. iIntros (v) "!> #Hv !>". iFrame "Hv". Qed.
+
+  Lemma lty_le_mutexguard A1 A2 :
+    ▷ (A1 <:> A2) -∗
+    mutexguard A1 <: mutexguard A2.
+  Proof.
+    iIntros "#[Hle1 Hle2]" (v) "!>".
+    iDestruct 1 as (γ l lk w ->) "[Hinv [Hlock Hinner]]".
+    iExists γ, l, lk, w. iSplit; first done.
+    iFrame "Hlock Hinner". iApply (spin_lock.is_lock_iff with "Hinv").
+    iIntros "!> !>". iSplit.
+    - iDestruct 1 as (v) "[Hl HA]". iExists v. iFrame "Hl". by iApply "Hle1".
+    - iDestruct 1 as (v) "[Hl HA]". iExists v. iFrame "Hl". by iApply "Hle2".
+  Qed.
+
+  Lemma lty_le_chan S1 S2 :
+    ▷ (S1 <: S2) -∗ chan S1 <: chan S2.
+  Proof.
+    iIntros "#Hle" (v) "!> H".
+    iApply (iProto_mapsto_le with "H [Hle]"). eauto.
+  Qed.
+
+  (** Session subtyping *)
+  Lemma lty_le_send A1 A2 S1 S2 :
+    ▷ (A2 <: A1) -∗ ▷ (S1 <: S2) -∗
+    (<!!> A1 ; S1) <: (<!!> A2 ; S2).
+  Proof.
+    iIntros "#HAle #HSle !>". iApply iProto_le_send; iIntros "!> /=" (x) "H".
+    iDestruct ("HAle" with "H") as "H".
+    eauto with iFrame.
+  Qed.
+
+  Lemma lty_le_recv A1 A2 S1 S2 :
+    ▷ (A1 <: A2) -∗ ▷ (S1 <: S2) -∗
+    (<??> A1 ; S1) <: (<??> A2 ; S2).
+  Proof.
+    iIntros "#HAle #HSle !>". iApply iProto_le_recv; iIntros "!> /=" (x) "H".
+    iDestruct ("HAle" with "H") as "H".
+    eauto with iFrame.
+  Qed.
+
+  Lemma lty_le_swap A1 A2 S :
+    ⊢ (<??> A1; <!!> A2; S) <: (<!!> A2; <??> A1; S).
+  Proof.
+    iIntros "!>". iApply iProto_le_swap. iIntros "!>" (v1 v2) "/= HS1 HS2".
+    iExists _, _,
+      (tele_app (TT:=[tele _]) (λ v2, (v2, ltty_car A2 v2, lsty_car S))),
+      (tele_app (TT:=[tele _]) (λ v1, (v1, ltty_car A1 v1, lsty_car S))),
+      v2, v1; simpl.
+    do 2 (iSplit; [done|]).
+    iFrame "HS1 HS2".
+    do 2 (iSplitR; [iApply iProto_le_refl|]). by iFrame.
+  Qed.
+
+  Lemma lty_le_select (Ss1 Ss2 : gmap Z (lsty Σ)) :
+    ▷ ([∗ map] S1;S2 ∈ Ss1; Ss2, S1 <: S2) -∗
+    lty_select Ss1 <: lty_select Ss2.
+  Proof.
+    iIntros "#H1 !>". iApply iProto_le_send; iIntros "!>" (x Hsome).
+    iExists x. iSplit; first done. iSplit.
+    - iDestruct (big_sepM2_forall with "H1") as "[% _]".
+      iPureIntro. naive_solver.
+    - iDestruct (big_sepM2_forall with "H1") as "[% H]".
+      iApply ("H" with "[] []").
+      + iPureIntro. apply lookup_lookup_total; naive_solver.
+      + iPureIntro. by apply lookup_lookup_total.
+  Qed.
+  Lemma lty_le_select_subseteq (Ss1 Ss2 : gmap Z (lsty Σ)) :
+    Ss2 ⊆ Ss1 →
+    ⊢ lty_select Ss1 <: lty_select Ss2.
+  Proof.
+    iIntros (Hle) "!>". iApply iProto_le_send; iIntros "!>" (x Hsome).
+    iExists _. iSplit; first done. iSplit.
+    { iPureIntro. by eapply lookup_weaken_is_Some. }
+    destruct Hsome as [P H1].
+    assert (Ss1 !! x = Some P) by eauto using lookup_weaken.
+    rewrite (lookup_total_correct Ss1 x P) //.
+    rewrite (lookup_total_correct Ss2 x P) //.
+    iApply iProto_le_refl.
+  Qed.
+
+  Lemma lty_le_branch (Ss1 Ss2 : gmap Z (lsty Σ)) :
+    ▷ ([∗ map] S1;S2 ∈ Ss1; Ss2, S1 <: S2) -∗
+    lty_branch Ss1 <: lty_branch Ss2.
+  Proof.
+    iIntros "#H1 !>". iApply iProto_le_recv; iIntros "!>" (x Hsome).
+    iExists x. iSplit; first done. iSplit.
+    - iDestruct (big_sepM2_forall with "H1") as "[% _]".
+      iPureIntro. by naive_solver.
+    - iDestruct (big_sepM2_forall with "H1") as "[% H]".
+      iApply ("H" with "[] []").
+      + iPureIntro. by apply lookup_lookup_total.
+      + iPureIntro. by apply lookup_lookup_total; naive_solver.
+  Qed.
+  Lemma lty_le_branch_subseteq (Ss1 Ss2 : gmap Z (lsty Σ)) :
+    Ss1 ⊆ Ss2 →
+    ⊢ lty_branch Ss1 <: lty_branch Ss2.
+  Proof.
+    iIntros (Hle) "!>". iApply iProto_le_recv; iIntros "!>" (x Hsome).
+    iExists _. iSplit; first done. iSplit.
+    { iPureIntro. by eapply lookup_weaken_is_Some. }
+    destruct Hsome as [P ?].
+    assert (Ss2 !! x = Some P) by eauto using lookup_weaken.
+    rewrite (lookup_total_correct Ss1 x P) //.
+    rewrite (lookup_total_correct Ss2 x P) //.
+    iApply iProto_le_refl.
+  Qed.
+
+  (** Algebraic laws *)
+  Lemma lty_le_app S11 S12 S21 S22 :
+    (S11 <: S21) -∗ (S12 <: S22) -∗
+    (S11 <++> S12) <: (S21 <++> S22).
+  Proof. iIntros "#H1 #H2 !>". by iApply iProto_le_app. Qed.
+
+  Lemma lty_le_app_id_l S : ⊢ (END <++> S) <:> S.
+  Proof. rewrite /lty_app left_id. iSplit; iModIntro; iApply iProto_le_refl. Qed.
+  Lemma lty_le_app_id_r S : ⊢ (S <++> END) <:> S.
+  Proof. rewrite /lty_app right_id. iSplit; iModIntro; iApply iProto_le_refl. Qed.
+  Lemma lty_le_app_assoc S1 S2 S3 :
+    ⊢ (S1 <++> S2) <++> S3 <:> S1 <++> (S2 <++> S3).
+  Proof. rewrite /lty_app assoc. iSplit; iModIntro; iApply iProto_le_refl. Qed.
+
+  Lemma lty_le_app_send A S1 S2 : ⊢ (<!!> A; S1) <++> S2 <:> (<!!> A; S1 <++> S2).
+  Proof.
+    rewrite /lty_app iProto_app_message_tele.
+    iSplit; iIntros "!>"; iApply iProto_le_refl.
+  Qed.
+  Lemma lty_le_app_recv A S1 S2 : ⊢ (<??> A; S1) <++> S2 <:> (<??> A; S1 <++> S2).
+  Proof.
+    rewrite /lty_app iProto_app_message_tele.
+    iSplit; iIntros "!>"; iApply iProto_le_refl.
+  Qed.
+
+  Lemma lty_le_app_choice a (Ss : gmap Z (lsty Σ)) S2 :
+    ⊢ lty_choice a Ss <++> S2 <:> lty_choice a ((.<++> S2) <$> Ss)%lty.
+  Proof.
+    destruct a.
+    - rewrite /lty_app iProto_app_message_tele. iSplit; iIntros "!> /=".
+      + iApply iProto_le_send; iIntros "!>" (x [S HSs]); simpl in *.
+        move: HSs; rewrite lookup_fmap fmap_Some; intros (S'&HSs&->).
+        iExists _; do 2 (iSplit; [by eauto|]).
+        rewrite !lookup_total_alt lookup_fmap !HSs /=. iApply iProto_le_refl.
+      + iApply iProto_le_send; iIntros "!>" (x [S HSs]); simpl in *.
+        iExists _; iSplit; [by eauto|].
+        rewrite !lookup_total_alt lookup_fmap !HSs /=.
+        iSplit; [by eauto|]. iApply iProto_le_refl.
+    - rewrite /lty_app iProto_app_message_tele. iSplit; iIntros "!> /=".
+      + iApply iProto_le_recv; iIntros "!>" (x [S HSs]); simpl in *.
+        iExists _; iSplit; [by eauto|].
+        rewrite !lookup_total_alt lookup_fmap !HSs /=.
+        iSplit; [by eauto|]. iApply iProto_le_refl.
+      + iApply iProto_le_recv; iIntros "!>" (x [S HSs]); simpl in *.
+        move: HSs; rewrite lookup_fmap fmap_Some; intros (S'&HSs&->).
+        iExists _; iSplit; [by eauto|].
+        rewrite !lookup_total_alt lookup_fmap !HSs /=.
+        iSplit; [by eauto|]. iApply iProto_le_refl.
+  Qed.
+  Lemma lty_le_app_select A Ss S2 :
+    ⊢ lty_select Ss <++> S2 <:> lty_select ((.<++> S2) <$> Ss)%lty.
+  Proof. apply lty_le_app_choice. Qed.
+  Lemma lty_le_app_branch A Ss S2 :
+    ⊢ lty_branch Ss <++> S2 <:> lty_branch ((.<++> S2) <$> Ss)%lty.
+  Proof. apply lty_le_app_choice. Qed.
+
+  Lemma lty_le_dual S1 S2 : S2 <: S1 -∗ lty_dual S1 <: lty_dual S2.
+  Proof. iIntros "#H !>". by iApply iProto_le_dual. Qed.
+  Lemma lty_le_dual_l S1 S2 : lty_dual S2 <: S1 -∗ lty_dual S1 <: S2.
+  Proof. iIntros "#H !>". by iApply iProto_le_dual_l. Qed.
+  Lemma lty_le_dual_r S1 S2 : S2 <: lty_dual S1 -∗ S1 <: lty_dual S2.
+  Proof. iIntros "#H !>". by iApply iProto_le_dual_r. Qed.
+
+  Lemma lty_le_dual_end : ⊢ lty_dual (Σ:=Σ) END <:> END.
+  Proof. rewrite /lty_dual iProto_dual_end=> /=. apply lty_bi_le_refl. Qed.
+
+  Lemma lty_le_dual_message a A S :
+    ⊢ lty_dual (lty_message a A S) <:> lty_message (action_dual a) A (lty_dual S).
+  Proof.
+    iSplit; iIntros "!>"; rewrite /lty_dual iProto_dual_message_tele;
+      iApply iProto_le_refl.
+  Qed.
+  Lemma lty_le_dual_send A S : ⊢ lty_dual (<!!> A; S) <:> (<??> A; lty_dual S).
+  Proof. apply lty_le_dual_message. Qed.
+  Lemma lty_le_dual_recv A S : ⊢ lty_dual (<??> A; S) <:> (<!!> A; lty_dual S).
+  Proof. apply lty_le_dual_message. Qed.
+
+  Lemma lty_le_dual_choice a (Ss : gmap Z (lsty Σ)) :
+    ⊢ lty_dual (lty_choice a Ss) <:> lty_choice (action_dual a) (lty_dual <$> Ss).
+  Proof.
+    destruct a.
+    - rewrite /lty_dual iProto_dual_message_tele. iSplit; iIntros "!> /=".
+      + iApply iProto_le_recv; iIntros "!>" (x [S HSs]); simpl in *.
+        iExists _; iSplit; [by eauto|].
+        rewrite !lookup_total_alt lookup_fmap !HSs /=.
+        iSplit; [by eauto|]. iApply iProto_le_refl.
+      + iApply iProto_le_recv; iIntros "!>" (x [S HSs]); simpl in *.
+        move: HSs; rewrite lookup_fmap fmap_Some; intros (S'&HSs&->).
+        iExists _; iSplit; [by eauto|].
+        rewrite !lookup_total_alt lookup_fmap !HSs /=.
+        iSplit; [by eauto|]. iApply iProto_le_refl.
+    - rewrite /lty_dual iProto_dual_message_tele. iSplit; iIntros "!> /=".
+      + iApply iProto_le_send; iIntros "!>" (x [S HSs]); simpl in *.
+        move: HSs; rewrite lookup_fmap fmap_Some; intros (S'&HSs&->).
+        iExists _; do 2 (iSplit; [by eauto|]).
+        rewrite !lookup_total_alt lookup_fmap !HSs /=. iApply iProto_le_refl.
+      + iApply iProto_le_send; iIntros "!>" (x [S HSs]); simpl in *.
+        iExists _; iSplit; [by eauto|].
+        rewrite !lookup_total_alt lookup_fmap !HSs /=.
+        iSplit; [by eauto|]. iApply iProto_le_refl.
+  Qed.
+
+  Lemma lty_le_dual_select (Ss : gmap Z (lsty Σ)) :
+    ⊢ lty_dual (lty_select Ss) <:> lty_branch (lty_dual <$> Ss).
+  Proof. iApply lty_le_dual_choice. Qed.
+  Lemma lty_le_dual_branch (Ss : gmap Z (lsty Σ)) :
+    ⊢ lty_dual (lty_branch Ss) <:> lty_select (lty_dual <$> Ss).
+  Proof. iApply lty_le_dual_choice. Qed.
+End subtyping_rules.
