theories/logrel/typing_judgment.v
@@ -1,0 +1,41 @@
+From iris.heap_lang Require Import metatheory adequacy.
+From actris.logrel Require Export term_types.
+From actris.logrel Require Import environments.
+From iris.proofmode Require Import tactics.
+
+(* The semantic typing judgement *)
+Definition ltyped `{!heapG Σ}
+    (Γ Γ' : gmap string (ltty Σ)) (e : expr) (A : ltty Σ) : iProp Σ :=
+  (■ ∀ vs, env_ltyped Γ vs -∗
+           WP subst_map vs e {{ v, ltty_car A v ∗ env_ltyped Γ' vs }})%I.
+
+Notation "Γ ⊨ e : A ⫤ Γ'" := (ltyped Γ Γ' e A)
+  (at level 100, e at next level, A at level 200).
+Notation "Γ ⊨ e : A" := (Γ ⊨ e : A ⫤ Γ)
+  (at level 100, e at next level, A at level 200).
+
+Lemma ltyped_frame `{!heapG Σ} (Γ Γ' Γ1 Γ1' Γ2 : gmap string (ltty Σ)) e A :
+  env_split Γ Γ1 Γ2 -∗
+  env_split Γ' Γ1' Γ2 -∗
+  (Γ1 ⊨ e : A ⫤ Γ1') -∗
+  Γ ⊨ e : A ⫤ Γ'.
+Proof.
+  iIntros "#Hsplit #Hsplit' #Htyped !>" (vs) "Henv".
+  iDestruct ("Hsplit" with "Henv") as "[Henv1 Henv2]".
+  iApply (wp_wand with "(Htyped Henv1)").
+  iIntros (v) "[$ Henv1']".
+  iApply "Hsplit'". iFrame "Henv1' Henv2".
+Qed.
+
+Lemma ltyped_safety `{heapPreG Σ} e σ es σ' e' :
+  (∀ `{heapG Σ}, ∃ A Γ', ⊢ ∅ ⊨ e : A ⫤ Γ') →
+  rtc erased_step ([e], σ) (es, σ') → e' ∈ es →
+  is_Some (to_val e') ∨ reducible e' σ'.
+Proof.
+  intros Hty. apply (heap_adequacy Σ NotStuck e σ (λ _, True))=> // ?.
+  destruct (Hty _) as (A & Γ' & He).
+  iDestruct (He) as "He".
+  iSpecialize ("He" $!∅).
+  iSpecialize ("He" with "[]"); first by rewrite /env_ltyped.
+  iEval (rewrite -(subst_map_empty e)). iApply (wp_wand with "He"); auto.
+Qed.
